proof/correctness/avx2/Fq_avx2.ec
@@ -2,7 +2,7 @@ require import AllCore List Int IntDiv CoreMap Real Number.
 from Jasmin require import JModel JWord.
 require import Fq Array16 Array16p.
 require import W16extra WArray512 WArray32 WArray16.
-require import Ops.
+require import AVX2_Ops.
 require import List_hakyber.
 require import KyberCPA_avx2.
 require import KyberPoly_avx2_prevec.
